Thread through a state interpretation for the FFI
In theory this should allow us to actually write propositions over the
FFI state, using any camera for the relevant resources. We need decent
flexibility since we'll instantiate the FFI for a disk, file system, and
applications.

src/go_lang/adequacy.v
@@ -5,25 +5,43 @@ From iris.program_logic Require Export weakestpre adequacy.
 From Perennial.go_lang Require Import proofmode notation.
 Set Default Proof Using "Type".
 
-Class heapPreG `{ffi_sem: ext_semantics} Σ := HeapPreG {
+Class ffi_interp_adequacy `{!ffi_interp ffi} :=
+  { ffi_preG: gFunctors -> Type;
+    ffiΣ: gFunctors;
+    (* modeled after subG_gen_heapPreG and gen_heap_init *)
+    subG_ffiPreG : forall Σ, subG ffiΣ Σ -> ffi_preG Σ;
+    ffi_init : forall Σ, ffi_preG Σ -> forall (σ:ffi_state),
+(|==> ∃ (H0: ffiG Σ), ffi_ctx H0 σ)%I;
+  }.
+
+(* this is the magic that lets subG_ffiPreG solve for an ffi_preG using only
+typeclass resolution, which is the one thing solve_inG tries. *)
+Existing Class ffi_preG.
+Hint Resolve subG_ffiPreG : typeclass_instances.
+
+Class heapPreG `{ext: ext_op} `{ffi_interp_adequacy} Σ := HeapPreG {
   heap_preG_iris :> invPreG Σ;
   heap_preG_heap :> gen_heapPreG loc val Σ;
-  heap_preG_proph :> proph_mapPreG proph_id (val * val) Σ
+  heap_preG_proph :> proph_mapPreG proph_id (val * val) Σ;
+  heap_preG_ffi : ffi_preG Σ;
 }.
 
-Definition heapΣ `{ffi_sem: ext_semantics} : gFunctors := #[invΣ; gen_heapΣ loc val; proph_mapΣ proph_id (val * val)].
-Instance subG_heapPreG `{ffi_sem: ext_semantics} {Σ} : subG heapΣ Σ → heapPreG Σ.
+Hint Resolve heap_preG_ffi : typeclass_instances.
+
+Definition heapΣ `{ext: ext_op} `{ffi_interp_adequacy} : gFunctors := #[invΣ; gen_heapΣ loc val; ffiΣ; proph_mapΣ proph_id (val * val)].
+Instance subG_heapPreG `{ext: ext_op} `{ffi_interp_adequacy} {Σ} : subG heapΣ Σ → heapPreG Σ.
 Proof. solve_inG. Qed.
 
-Definition heap_adequacy `{ffi_sem: ext_semantics} Σ `{!heapPreG Σ} s e σ φ :
+Definition heap_adequacy `{ffi_sem: ext_semantics} `{!ffi_interp ffi} {Hffi_adequacy:ffi_interp_adequacy} Σ `{!heapPreG Σ} s e σ φ :
   (∀ `{!heapG Σ}, WP e @ s; ⊤ {{ v, ⌜φ v⌝ }}%I) →
   adequate s e σ (λ v _, φ v).
 Proof.
   intros Hwp; eapply (wp_adequacy _ _); iIntros (??) "".
   iMod (gen_heap_init σ.(heap)) as (?) "Hh".
   iMod (proph_map_init κs σ.(used_proph_id)) as (?) "Hp".
+  iMod (ffi_init _ _ σ.(world)) as (HffiG) "Hw".
   iModIntro. iExists
-    (λ σ κs, (gen_heap_ctx σ.(heap) ∗ proph_map_ctx κs σ.(used_proph_id))%I),
+    (λ σ κs, (gen_heap_ctx σ.(heap) ∗ proph_map_ctx κs σ.(used_proph_id) ∗ ffi_ctx HffiG σ.(world))%I),
     (λ _, True%I).
-  iFrame. iApply (Hwp (HeapG _ _ _ _)).
+  iFrame. iApply (Hwp (HeapG _ _ _ _ _)).
 Qed.
