src/go_lang/lib/lock.v
@@ -2,7 +2,7 @@ From iris.base_logic.lib Require Export invariants.
 From Perennial.go_lang Require Export lifting notation.
 Set Default Proof Using "Type".
 
-Structure lock `{ffi_sem: ext_semantics} Σ `{!heapG Σ} := Lock {
+Structure lock `{ffi_sem: ext_semantics} `{!ffi_interp ffi} Σ `{!heapG Σ} := Lock {
   (* -- operations -- *)
   newlock : val;
   acquire : val;
@@ -26,13 +26,13 @@ Structure lock `{ffi_sem: ext_semantics} Σ `{!heapG Σ} := Lock {
     {{{ is_lock N γ lk R ∗ locked γ ∗ R }}} release lk {{{ RET #(); True }}}
 }.
 
-Arguments newlock {_ _ _ _ _} l.
-Arguments acquire {_ _ _ _ _} l.
-Arguments release {_ _ _ _ _} l.
-Arguments is_lock {_ _ _ _ _} l _ _ _ _.
-Arguments locked {_ _ _ _ _} l _.
+Arguments newlock {_ _ _ _ _ _} l.
+Arguments acquire {_ _ _ _ _ _} l.
+Arguments release {_ _ _ _ _ _} l.
+Arguments is_lock {_ _ _ _ _ _} l _ _ _ _.
+Arguments locked {_ _ _ _ _ _} l _.
 
 Existing Instances is_lock_ne is_lock_persistent locked_timeless.
 
-Instance is_lock_proper `{ffi_sem: ext_semantics} Σ `{!heapG Σ} (L: lock Σ) N γ lk:
+Instance is_lock_proper `{ffi_sem: ext_semantics} `{!ffi_interp ffi} Σ `{!heapG Σ} (L: lock Σ) N γ lk:
   Proper ((≡) ==> (≡)) (is_lock L N γ lk) := ne_proper _.
