src/go_lang/disk.v
@@ -62,4 +62,14 @@ Section semantics.
 
   .
 
+  (*
+  Lemma wp_Read s E a q v :
+    {{{ ▷ l ↦{q} v }}} ExternalOp Read (Val $ LitV $ LitInt a) @ s; E {{{ RET v; l ↦{q} v }}}.
+  Proof.
+    iIntros (Φ) ">Hl HΦ". iApply wp_lift_atomic_head_step_no_fork; auto.
+    iIntros (σ1 κ κs n) "[Hσ Hκs] !>". iDestruct (@gen_heap_valid with "Hσ Hl") as %?.
+    iSplit; first by eauto. iNext; iIntros (v2 σ2 efs Hstep); inv_head_step.
+    iModIntro; iSplit=> //. iFrame. by iApply "HΦ".
+  Qed. *)
+
 End semantics.
