src/go_lang/total_adequacy.v
@@ -4,16 +4,17 @@ From Perennial.go_lang Require Export adequacy.
 From Perennial.go_lang Require Import proofmode notation.
 Set Default Proof Using "Type".
 
-Definition heap_total `{ffi_sem: ext_semantics} Σ `{!heapPreG Σ} s e σ φ :
+Definition heap_total `{ffi_sem: ext_semantics} `{!ffi_interp ffi} `{!ffi_interp_adequacy} Σ `{!heapPreG Σ} s e σ φ :
   (∀ `{!heapG Σ}, WP e @ s; ⊤ [{ v, ⌜φ v⌝ }]%I) →
   sn erased_step ([e], σ).
 Proof.
   intros Hwp; eapply (twp_total _ _); iIntros (?) "".
   iMod (gen_heap_init σ.(heap)) as (?) "Hh".
   iMod (proph_map_init [] σ.(used_proph_id)) as (?) "Hp".
+  iMod (ffi_init _ _ σ.(world)) as (HffiG) "Hw".
   iModIntro.
   iExists
-    (λ σ κs _, (gen_heap_ctx σ.(heap) ∗ proph_map_ctx κs σ.(used_proph_id))%I),
+    (λ σ κs _, (gen_heap_ctx σ.(heap) ∗ proph_map_ctx κs σ.(used_proph_id) ∗ ffi_ctx HffiG σ.(world))%I),
     (λ _, True%I); iFrame.
-  iApply (Hwp (HeapG _ _ _ _)).
+  iApply (Hwp (HeapG _ _ _ _ _)).
 Qed.
